verif/trie/bordernode_fun.v
@@ -1,0 +1,141 @@
+(** * bordernode_fun.v : Functional Model of BorderNode*)
+Require Import VST.floyd.functional_base.
+Require Import common.
+Require Import keyslice_fun.
+
+Module BorderNode (ValueType: VALUE_TYPE).
+  Definition prefix_key := Z.
+  Definition suffix_key := string.
+  Definition value := ValueType.type.
+  Definition default_val := ValueType.default.
+  
+  Definition store: Type := list value * option (string * value).
+  
+  Definition empty: store := (list_repeat (Z.to_nat keyslice_length) default_val, None).
+
+  Instance inhabitant_value: Inhabitant value := ValueType.inhabitant_value.
+  Definition get_prefix (k: prefix_key) (s: store): value :=
+    let (prefixes, _) := s in
+    Znth k prefixes.
+
+  Definition get_suffix (k: suffix_key) (s: store): value :=
+    match s with
+    | (_, Some (s, v)) =>
+      if eq_dec k s then v else default_val
+    | _ => default_val
+    end.
+
+  Definition put_prefix (k: prefix_key) (v: value) (s: store): store :=
+    let (prefixes, suffix) := s in
+    (upd_Znth k prefixes v, suffix).
+
+  Definition put_suffix (k: suffix_key) (v: value) (s: store): store :=
+    let (prefixes, _) := s in
+    (prefixes, Some (k, v)).
+
+  Definition invariant (s: store) := let (prefixes, _) := s in Zlength prefixes = keyslice_length.
+
+  Lemma empty_invariant: invariant empty.
+  Proof.
+    simpl.
+    rewrite Zlength_list_repeat; rep_omega.
+  Qed.
+
+  Lemma get_prefix_empty: forall k,
+      0 <= k < keyslice_length -> get_prefix k empty = default_val.
+  Proof.
+    intros.
+    simpl. 
+    rewrite Znth_list_repeat_inrange by assumption.
+    reflexivity.
+  Qed.
+
+  Lemma get_suffix_empty: forall k,
+      get_suffix k empty = default_val.
+  Proof.
+    intros.
+    simpl. 
+    reflexivity.
+  Qed.
+
+  Lemma put_prefix_invariant: forall k v s,
+      invariant s -> 0 <= k < keyslice_length -> invariant (put_prefix k v s).
+  Proof.
+    intros.
+    destruct s.
+    simpl in *.
+    rewrite upd_Znth_Zlength by list_solve.
+    assumption.
+  Qed.
+
+  Lemma put_suffix_invariant: forall k v s,
+      invariant s -> invariant (put_suffix k v s).
+  Proof.
+    intros.
+    destruct s.
+    simpl in *.
+    assumption.
+  Qed.
+
+  Lemma get_put_prefix_same: forall k v s,
+      invariant s -> 0 <= k < keyslice_length -> get_prefix k (put_prefix k v s) = v.
+  Proof.
+    intros.
+    destruct s.
+    simpl in *.
+    rewrite upd_Znth_same by list_solve.
+    reflexivity.
+  Qed.
+
+  Lemma get_put_prefix_diff: forall k1 k2 v s,
+      invariant s -> 0 <= k1 < keyslice_length -> 0 <= k2 < keyslice_length -> k1 <> k2 ->
+      get_prefix k1 (put_prefix k2 v s) = get_prefix k1 s.
+  Proof.
+    intros.
+    destruct s.
+    simpl in *.
+    rewrite upd_Znth_diff by list_solve.
+    reflexivity.
+  Qed.
+
+  Lemma get_put_suffix_same: forall k v s,
+      get_suffix k (put_suffix k v s) = v.
+  Proof.
+    intros.
+    destruct s.
+    simpl.
+    rewrite if_true by auto.
+    reflexivity.
+  Qed.
+
+  Lemma get_put_suffix_diff: forall k1 k2 v s,
+      k1 <> k2 -> get_suffix k1 (put_suffix k2 v s) = default_val.
+  Proof.
+    intros.
+    destruct s.
+    simpl.
+    rewrite if_false by auto.
+    reflexivity.
+  Qed.
+
+  Lemma get_put_non_interference1: forall k1 k2 v s,
+      get_prefix k1 (put_suffix k2 v s) = get_prefix k1 s.
+  Proof.
+    intros.
+    destruct s; reflexivity.
+  Qed.
+
+  Lemma get_put_non_interference2: forall k1 k2 v s,
+      get_suffix k1 (put_prefix k2 v s) = get_suffix k1 s.
+  Proof.
+    intros.
+    destruct s; reflexivity.
+  Qed.
+
+  Hint Rewrite get_put_prefix_same: bordernode.
+  Hint Rewrite get_put_prefix_diff: bordernode.
+  Hint Rewrite get_put_prefix_same: bordernode.
+  Hint Rewrite get_put_suffix_diff: bordernode.
+  Hint Rewrite get_put_non_interference1: bordernode.
+  Hint Rewrite get_put_non_interference2: bordernode.
+End BorderNode.
