verif/trie/common.v
@@ -1,0 +1,10 @@
+(** * common.v : Common definitions *)
+Require Import VST.floyd.functional_base.
+Definition string := list byte.
+Instance EqDec_string: EqDec string := list_eq_dec Byte.eq_dec.
+
+Module Type VALUE_TYPE.
+  Parameter type: Type.
+  Parameter default: type.
+  Parameter inhabitant_value: Inhabitant type.
+End VALUE_TYPE.
