verif/trie/kv_fun.v
@@ -1,0 +1,20 @@
+(** * kvfun.v : Functional model KV Store *)
+Require Import VST.floyd.functional_base.
+
+Module Type KV_STORE.
+  Parameter store: Type.
+  Parameter key: Type.
+  Parameter value: Type.
+  Parameter default_val: value.
+  Parameter empty: store.
+  Parameter get: key -> store -> value.
+  Parameter put: key -> value -> store -> store.
+  Axiom get_empty: forall k,
+      get k empty = default_val.
+  Axiom get_put_same: forall k v s,
+      get k (put k v s) = v.
+  Axiom get_put_diff: forall k1 k2 v s,
+      k1 <> k2 -> get k1 (put k2 v s) = get k1 s.
+End KV_STORE.
+
+(* TODO: An functional implementation of [KV_STORE] *)
