verif/trie/specs.v
@@ -1,0 +1,155 @@
+(** * specs.v : Collection of all related specs *)
+Require Import VST.floyd.proofauto.
+Require Import VST.floyd.library.
+Require Import common.
+(* clight files *)
+Require Import surely_malloc.
+Require Import util.
+Require Import bordernode.
+Instance CompSpecs : compspecs. Proof. make_compspecs prog. Defined.
+Definition Vprog : varspecs. mk_varspecs prog. Defined.
+
+(* functional definitions *)
+Require Import keyslice_fun.
+Require Import bordernode_fun.
+
+Definition tbordernode: type := Tstruct _BorderNode noattr.
+
+Definition cstring_len (sh: share) (str: string) (s: val) :=
+  data_at sh (tarray tschar (Zlength str)) (map Vbyte (str)) s && !! (0 < Zlength str <= Int.max_unsigned).
+
+Module BorderNodeValue <: VALUE_TYPE.
+  Definition type := val.
+  Definition default := nullval.
+  Definition inhabitant_value := Vundef.
+End BorderNodeValue.
+
+Module BorderNode := BorderNode BorderNodeValue.
+
+Definition bordernode_rep (sh: share) (s: BorderNode.store) (p: val): mpred :=
+  let (prefixes, suffix_val) := s in
+  match suffix_val with
+  | Some (k, v) =>
+    EX p': val, EX sh_string: share,
+      data_at sh tbordernode (prefixes, (v, (p', Vint (Int.repr (Zlength k))))) p *
+      cstring_len sh_string k p' &&
+      !! (readable_share sh_string) && 
+      !! (Forall (fun p => is_pointer_or_null p) (prefixes)) &&
+      !! (is_pointer_or_null v)
+  | None =>
+    data_at sh tbordernode (prefixes, (nullval, (nullval, Vint Int.zero))) p &&
+    !! (Forall (fun p => is_pointer_or_null p) (prefixes))
+  end * malloc_token sh tbordernode p.
+
+(* Specification for [surely_malloc.c] *)
+
+Definition surely_malloc_spec: ident * funspec :=
+  DECLARE _surely_malloc
+  WITH t:type
+  PRE [ _n OF tuint ]
+    PROP (0 <= sizeof t <= Int.max_unsigned;
+          complete_legal_cosu_type t = true;
+          natural_aligned natural_alignment t = true)
+    LOCAL (temp _n (Vint (Int.repr (sizeof t))))
+    SEP ()
+  POST [ tptr tvoid ] EX p:_,
+    PROP ()
+    LOCAL (temp ret_temp p)
+    SEP (malloc_token Tsh t p * data_at_ Tsh t p).
+
+(* Specification for [util.c] *)
+
+Definition UTIL_GetNextKeySlice_spec: ident * funspec :=
+  DECLARE _UTIL_GetNextKeySlice
+  WITH sh: share, str: val, key: string
+  PRE [ _str OF tptr tschar, _len OF tint ]
+  PROP (readable_share sh;
+        0 <= Zlength key <= keyslice_length)
+  LOCAL (temp _str str;
+         temp _len (Vint (Int.repr (Zlength key))))
+  SEP (cstring_len sh key str)
+  POST [ (if Archi.ptr64 then tulong else tuint) ]
+  PROP ()
+  LOCAL (temp ret_temp (Vint (Int.repr (get_keyslice key)))) (* machine dependent spec *)
+  SEP (cstring_len sh key str).
+
+Definition UTIL_StrEqual_spec: ident * funspec :=
+  DECLARE _UTIL_StrEqual
+  WITH sh1: share, s1: val, str1: string,
+       sh2: share, s2: val, str2: string
+  PRE [ _a OF tptr tschar, _lenA OF tuint, _b OF tptr tschar, _lenB OF tuint ]
+  PROP (readable_share sh1;
+        readable_share sh2)
+  LOCAL (temp _a s1;
+         temp _lenA (Vint (Int.repr (Zlength str1)));
+         temp _b s2;
+         temp _lenB (Vint (Int.repr (Zlength str2))))
+  SEP (cstring_len sh1 str1 s1;
+       cstring_len sh2 str2 s2)
+  POST [ tint ]
+  PROP ()
+  LOCAL (temp ret_temp (Vint (if eq_dec str1 str2 then Int.one else Int.zero)))
+  SEP (cstring_len sh1 str1 s1;
+       cstring_len sh2 str2 s2).
+
+(* Specification for [bordernode.c] *)
+
+Definition BN_NewBorderNode_spec: ident * funspec :=
+  DECLARE _BN_NewBorderNode
+  WITH tt: unit
+  PRE [ ]
+  PROP ()
+  LOCAL ()
+  SEP ()
+  POST [ tptr tbordernode ] EX p:val,
+  PROP ()
+  LOCAL (temp ret_temp p)
+  SEP (bordernode_rep Tsh BorderNode.empty p).
+
+Definition BN_SetPrefixValue_spec: ident * funspec :=
+  DECLARE _BN_SetPrefixValue
+  WITH sh: share, key: Z, bordernode: BorderNode.store, p: val, value: val
+  PRE [ _bn OF tptr tbordernode, _i OF tint, _val OF tptr tvoid ]
+  PROP (0 <= key < keyslice_length;
+        writable_share sh)
+  LOCAL (temp _i (Vint (Int.repr key));
+         temp _bn p;
+         temp _val value)
+  SEP (bordernode_rep sh bordernode p)
+  POST [ tvoid ]
+  PROP ()
+  LOCAL ()
+  SEP (bordernode_rep sh (BorderNode.put_prefix key value bordernode) p).
+
+Definition BN_GetPrefixValue_spec: ident * funspec :=
+  DECLARE _BN_GetPrefixValue
+  WITH sh: share, key: Z, bordernode: BorderNode.store, p: val
+  PRE [ _bn OF tptr tbordernode, _i OF tint ]
+  PROP (0 <= key < keyslice_length;
+        readable_share sh)
+  LOCAL (temp _i (Vint (Int.repr key));
+         temp _bn p)
+  SEP (bordernode_rep sh bordernode p)
+  POST [ tptr tvoid ]
+  PROP ()
+  LOCAL (temp ret_temp (BorderNode.get_prefix key bordernode))
+  SEP (bordernode_rep sh bordernode p).
+
+Definition BN_GetSuffixValue_spec: ident * funspec :=
+  DECLARE _BN_GetSuffixValue
+  WITH sh_string: share, key: string, len: Z, s: val,
+       sh_bordernode: share, bordernode: BorderNode.store, p: val
+  PRE [ _bn OF tptr tbordernode, _suf OF tptr tschar, _len OF tuint ]
+  PROP (readable_share sh_string;
+        readable_share sh_bordernode;
+        Zlength key = len)
+  LOCAL (temp _bn p;
+         temp _suf s;
+         temp _len (Vint (Int.repr len)))
+  SEP (cstring_len sh_string key s;
+       bordernode_rep sh_bordernode bordernode p)
+  POST [ tptr tvoid ]
+  PROP ()
+  LOCAL (temp ret_temp (BorderNode.get_suffix key bordernode))
+  SEP (cstring_len sh_string key s;
+       bordernode_rep sh_bordernode bordernode p).
