verif/trie/verif_bordernode.v
@@ -1,0 +1,215 @@
+(** * verif_bordernode.v: Correctness proof of bordernode *)
+
+Require Import VST.floyd.proofauto.
+Require Import VST.floyd.library.
+Require Import bordernode.
+Require Import specs.
+
+Require Import common.
+Require Import bordernode_fun.
+Require Import keyslice_fun.
+
+Import Coq.Lists.List.ListNotations.
+
+Lemma Forall_upd_Znth {A: Type} {Inh: Inhabitant A}: forall (l: list A) (k: Z) (v: A) (P: A -> Prop),
+    0 <= k < Zlength l ->
+    Forall P l ->
+    P v ->
+    Forall P (upd_Znth k l v).
+Proof.
+  intros.
+  rewrite <- (sublist_same 0 (Zlength l) l) by reflexivity.
+  rewrite (sublist_split 0 k) by list_solve.
+  rewrite (sublist_split k (k + 1)) by list_solve.
+  rewrite upd_Znth_app2 by list_solve.
+  rewrite upd_Znth_app1 by list_solve.
+  do 2 rewrite Forall_app.
+  split3; try (apply Forall_sublist; assumption).
+  rewrite Zlength_sublist by list_solve.
+  replace (k - (k - 0)) with 0 by omega.
+  rewrite sublist_len_1 by list_solve.
+  rewrite upd_Znth0.
+  rewrite sublist_nil.
+  auto.
+Qed.
+
+Definition bordernode_rep_length_inv: forall sh s p,
+    bordernode_rep sh s p |-- !! (Zlength (fst s) = keyslice_length).
+Proof.
+  intros.
+  unfold bordernode_rep.
+  destruct s as [? [[] | ]].
+  - Intros p'.
+    Intros sh_string.
+    entailer!.
+    simplify_value_fits in H2.
+    destruct H2 as [? _].
+    simplify_value_fits in H2.
+    rep_omega.
+  - entailer!.
+    simplify_value_fits in H1.
+    destruct H1 as [? _].
+    simplify_value_fits in H1.
+    rep_omega.
+Qed.
+Hint Resolve bordernode_rep_length_inv: saturate_local.
+
+Definition Gprog : funspecs :=
+  ltac:(with_library prog [
+          surely_malloc_spec; UTIL_StrEqual_spec;
+          BN_NewBorderNode_spec; BN_SetPrefixValue_spec;
+          BN_GetPrefixValue_spec; BN_GetSuffixValue_spec
+       ]).
+
+Lemma body_BN_NewBorderNode: semax_body Vprog Gprog f_BN_NewBorderNode BN_NewBorderNode_spec.
+Proof.
+  start_function.
+  forward_call (tbordernode).
+  split3; auto; simpl; rep_omega.
+  Intros p.
+  forward_for_simple_bound (keyslice_length) (EX i: Z,
+    PROP (0 <= i <= keyslice_length)
+    LOCAL (temp _bordernode p)
+    SEP (malloc_token Tsh tbordernode p;
+         data_at Tsh tbordernode (list_repeat (Z.to_nat i) nullval ++ list_repeat (Z.to_nat (keyslice_length - i)) Vundef, (Vundef, (Vundef, Vundef))) p))%assert.
+  entailer!.
+  unfold_data_at 1%nat.
+  unfold data_at_.
+  unfold field_at_.
+  unfold_field_at 1%nat.
+  entailer!.
+  - forward.
+    entailer!.
+    rewrite <- list_repeat_app' by list_solve.
+    rewrite upd_Znth_app2 by list_solve.
+    rewrite Zlength_list_repeat by list_solve.
+    rewrite Z.sub_diag.
+    simpl.
+    rewrite upd_Znth0.
+    rewrite sublist_list_repeat by list_solve.
+    rewrite Zlength_list_repeat by list_solve.
+    rewrite <- app_assoc.
+    rewrite semax_lemmas.cons_app.
+    replace (keyslice_length  - (i + 1)) with (keyslice_length - i - 1) by rep_omega.
+    entailer!.
+  - forward.
+    forward.
+    forward.
+    forward.
+    Exists p.
+    rewrite Z.sub_diag.
+    simpl.
+    rewrite app_nil_r.
+    entailer!.
+    apply Forall_list_repeat.
+    auto.
+Qed.
+
+Lemma body_BN_SetPrefixValue: semax_body Vprog Gprog f_BN_SetPrefixValue BN_SetPrefixValue_spec.
+Proof.
+  start_function.
+  forward_if (True); [(forward; entailer!) | rep_omega | ]; Intros.
+  forward_if (True); [(forward; entailer!) | rep_omega | ]; Intros.
+  assert_PROP (Zlength (fst bordernode) = keyslice_length). {
+    entailer!.
+  }
+  unfold bordernode_rep.
+  destruct bordernode as [? [[]|]]; simpl in H0.
+  - Intros p'.
+    Intros sh_string.
+    forward.
+    forward.
+    Exists p'.
+    Exists sh_string.
+    entailer!.
+    apply Forall_upd_Znth; first [list_solve | assumption].
+  - Intros.
+    forward.
+    forward.
+    entailer!.
+    apply Forall_upd_Znth; first [list_solve | assumption].
+Qed.
+
+Lemma body_BN_GetPrefixValue: semax_body Vprog Gprog f_BN_GetPrefixValue BN_GetPrefixValue_spec.
+Proof.
+  start_function.
+  forward_if (True); [(forward; entailer!) | rep_omega | ]; Intros.
+  forward_if (True); [(forward; entailer!) | rep_omega | ]; Intros.
+  assert_PROP (Zlength (fst bordernode) = keyslice_length). {
+    entailer!.
+  }
+  unfold bordernode_rep.
+  destruct bordernode as [? [[] | ]]; simpl in H0.
+  - Intros p'.
+    Intros sh_string'.
+    forward.
+    + entailer!.
+      apply Forall_Znth.
+      * rep_omega.
+      * assumption.
+    + forward.
+      Exists p'.
+      Exists sh_string'.
+      entailer!.
+  - Intros.
+    forward.
+    + entailer!.
+      apply Forall_Znth.
+      * rep_omega.
+      * assumption.
+    + forward.
+Qed.
+
+Lemma body_BN_GetSuffixValue: semax_body Vprog Gprog f_BN_GetSuffixValue BN_GetSuffixValue_spec.
+Proof.
+  start_function.
+  unfold bordernode_rep.
+  destruct bordernode as [? [[] |]].
+  - Intros p'.
+    unfold cstring_len.
+    Intros sh_string'.
+    forward.
+    forward_if (p' <> nullval).
+    (* entailer! does not solve the type check here *)
+    apply denote_tc_test_eq_split; first [entailer!].
+    assert (data_at sh_string' (tarray tschar (Zlength s0)) (map Vbyte s0) p' |-- valid_pointer p'). {
+      apply data_at_valid_ptr.
+      auto.
+      simpl.
+      rewrite Z.mul_1_l.
+      rewrite Z.max_r by rep_omega.
+      rep_omega.
+    }
+    entailer!.
+    + assert_PROP (False). { entailer!. }
+      contradiction.
+    + forward.
+      entailer!.
+    + forward.
+      forward.
+      forward_call (sh_string, s, key, sh_string', p', s0).
+      entailer!. (* I don't know what's this goal *)
+      unfold cstring_len.
+      entailer!.
+      forward_if.
+      * if_tac in H5; [ | contradiction].
+        forward.
+        forward.
+        Exists p'.
+        Exists sh_string'.
+        rewrite if_true by auto.
+        entailer!.
+      * if_tac in H5; [discriminate H5 | ].
+        forward.
+        Exists p'.
+        Exists sh_string'.
+        rewrite if_false by auto.
+        entailer!.
+  - Intros.
+    forward.
+    forward_if (nullval <> nullval).
+    + forward.
+    + discriminate H1.
+    + Intros.
+      contradiction.
+Qed.
